Reflection/Test/CMonExpTest.v
@@ -19,21 +19,9 @@ Proof. cmon_simpl. reflexivity. Qed.
 Goal op a b = op b a.
 Proof. cmon_simpl. reflexivity. Qed.
 
+(* Other tests. *)
 Goal op a (op (op b c) (op d (op (op e e) d))) =
      op (op a d) (op d (op c (op e (op e b)))).
-Proof. cmon_simpl. reflexivity. Qed.
-
-(* Other tests. *)
-Goal b = b' -> op a (op b c) = op (op a b') c.
-Proof. solveGoal. Qed.
-
-Goal op a b = op a b' -> op (op a b) c = op b' (op a c).
-Proof.
-  cmon_simpl. rewrite ?assoc. rewrite (comm b').
-  rewrite <- !H. cmon_simpl. reflexivity.
-Qed.
-
-Goal a = b -> b = c -> c = a -> op b (op a c) = op a (op neutr (op b c)).
 Proof. cmon_simpl. reflexivity. Qed.
 
 End Test.
