Reflection/Test/CMonFormulaTest.v
@@ -1,0 +1,32 @@
+Add Rec LoadPath "/home/zeimer/Code/Coq".
+
+Require Import CMonRefl.
+
+Section Test.
+
+Variable (X : CMon) (a a' b b' c c' d e f : X).
+Variable P Q R S : Prop.
+
+Goal a = a.
+Proof. solveGoal. Qed.
+
+Goal a = b -> b = a.
+Proof. solveGoal. Qed.
+
+Goal a = b -> b = c -> a = c.
+Proof. solveGoal. Abort.
+
+Goal b = c -> a = b -> a = c.
+Proof. solveGoal. Qed.
+
+Goal b = b' -> op a (op b c) = op (op a b') c.
+Proof. solveGoal. solveGoal. cmon_simpl. Print Ltac cmon_simpl'. solveGoal. cbn. Abort.
+
+Goal op a b = op a b' -> op (op a b) c = op b' (op a c).
+Proof.
+  cmon_simpl. rewrite ?assoc. rewrite (comm b').
+  rewrite <- !H. cmon_simpl. reflexivity.
+Qed.
+
+Goal a = b -> b = c -> c = a -> op b (op a c) = op a (op neutr (op b c)).
+Proof. cmon_simpl. reflexivity. Qed.
