Thrash/GenRec.v
@@ -1,0 +1,148 @@
+Add Rec LoadPath "/home/zeimer/Code/Coq".
+
+Require Import Arith.
+Require Import Omega.
+Require Import Recdef.
+
+Definition divF (f : nat -> forall k : nat, 0 < k -> nat)
+  (n k : nat) (H : 0 < k) : nat :=
+match le_lt_dec k n with
+    | left _ => S (f (n - k) k H)
+    | right _ => 0
+end.
+
+Arguments iter [A] _ _.
+
+Theorem divF_terminates :
+  forall (n k : nat) (H : 0 < k),
+    {v : nat | exists p : nat, forall n_iter : nat, p < n_iter ->
+      forall f : forall n k : nat, 0 < k -> nat,
+         iter n_iter divF f n k H = v}.
+Proof.
+  intros. generalize dependent n.
+  apply well_founded_induction_type with lt.
+    apply lt_wf.
+    intros. case_eq (le_lt_dec k x); intro.
+      Focus 2. exists 0. exists 0. intros. destruct n_iter; cbn.
+        omega.
+        unfold divF. rewrite H1. trivial.
+      destruct (H0 (x - k)) as [v Hv].
+        omega.
+        exists (S v). destruct Hv as [p Hp]. exists (S p). intros.
+          destruct (n_iter); cbn.
+            omega.
+            unfold divF. rewrite H1. f_equal. apply Hp. omega.
+Defined.
+
+Definition div (n k : nat) (H : 0 < k) : nat :=
+  proj1_sig (divF_terminates n k H).
+
+Require Import RCCBase.
+
+Theorem div_fix : div = divF div.
+Proof.
+  ext n; ext k; ext H.
+  unfold div at 1. destruct (divF_terminates n k H). cbn.
+  destruct e as [p Hp]. assert (p < S p) by omega.
+  rewrite <- (Hp _ H0 div). cbn. clear Hp. gen H; gen k; gen n.
+  induction p as [| p'].
+    trivial.
+    f_equal.
+Restart.
+  ext n. gen n. apply (@well_founded_induction _ _ lt_wf).
+  intros n IH. ext k; ext H. unfold divF.
+  case_eq (le_lt_dec k n); intros.
+    Focus 2. unfold div. destruct (divF_terminates _ _ _). cbn.
+      destruct e as [p Hp]. erewrite <- (Hp (S p)).
+        cbn. unfold divF. rewrite H0. trivial.
+        omega.
+    assert (n - k < n) by omega. specialize (IH _ H1).
+      assert (div (n - k) k H = divF div (n - k) k H). congruence. clear IH.
+      unfold divF in H2. case_eq (le_lt_dec k (n - k)); intros.
+        unfold div in *.
+        destruct (divF_terminates (n - k) k H),
+                 (divF_terminates n k H).
+Abort.
+
+Lemma div_equation :
+  forall (n k : nat) (H : 0 < k),
+    div n k H =
+    if le_lt_dec k n then S (div (n - k) k H) else 0.
+Proof.
+  intros. generalize dependent n.
+  apply (@well_founded_induction_type _ _ lt_wf); intros. unfold div.
+  destruct (divF_terminates x k H), (divF_terminates (x -k) k H); cbn.
+  destruct e as [p Hp], e0 as [p' Hp'].
+  case_eq (le_lt_dec k x); intros.
+    Focus 2. erewrite <- (Hp (S p)).
+      cbn. unfold divF. rewrite H1. trivial.
+      omega.
+    erewrite <- (Hp (S p)), <- (Hp' (S p')). case_eq (le_lt_dec k (x - k)); intros.
+      cbn. unfold divF. rewrite ?H1, ?H2. fold divF.
+      assert (x - k < x) by omega. specialize (H0 _ H3).
+      rewrite H2 in H0. unfold div in H0.
+        
+Restart.
+  intros. unfold div.
+  destruct (divF_terminates n k H),
+           (divF_terminates (n - k) k H); intros. cbn.
+  destruct e as [p Hp], e0 as [p' Hp'].
+  case_eq (le_lt_dec k n); intros; cbn.
+    Focus 2. erewrite <- (Hp (S p)).
+      cbn. unfold divF. rewrite H0. trivial.
+      omega.
+    case_eq (le_lt_dec p p'); intros.
+      assert (p < S (p + p')) by omega.
+        erewrite <- (Hp (S p')), <- (Hp' p'). cbn. unfold divF.
+        rewrite H0. fold divF. reflexivity.
+Restart.
+  intros. unfold div at 1. destruct (divF_terminates n k H). cbn.
+  case_eq (le_lt_dec k n); intros.
+    destruct e as [p Hp]. erewrite <- (Hp (S p)). cbn. unfold divF.
+      rewrite H0. fold divF. unfold div.
+      destruct (divF_terminates (n - k) k H). cbn. destruct e as [p' Hp'].
+        rewrite Hp'. all: auto. 
+Abort.
+
+Inductive divR' : nat -> nat -> nat -> Prop :=
+    | div_base :
+        forall (n k : nat), 0 < k -> n < k -> divR' n k 0
+    | div_rec :
+        forall (n k r : nat), 0 < k -> k <= n ->
+          divR' (n - k) k r -> divR' n k (S r).
+
+Hint Constructors divR'.
+
+Lemma divR'_correct :
+  forall (n k r : nat) (H : 0 < k),
+    div n k H = r -> divR' n k r.
+Proof.
+  apply (@well_founded_induction nat lt lt_wf
+    (fun n : nat => forall (k r : nat) (H : 0 < k ),
+      div n k H = r -> divR' n k r)).
+  intros. rewrite div_equation' in H1. destruct (le_lt_dec k x); subst.
+    Focus 2. constructor; auto.
+    constructor; auto. apply H with H0; omega.
+Qed.
+
+Lemma divR'_complete :
+  forall (n k r : nat) (H : 0 < k),
+    divR' n k r -> div n k H = r.
+Proof.
+  induction 1.
+    apply div_lt_n_k. assumption.
+    rewrite <- IHdivR' with H. rewrite div_le_k_n; auto.
+Qed.
+
+Theorem div_ind :
+  forall P : nat -> nat -> nat -> Prop,
+    (forall n k : nat, 0 < k -> n < k -> P n k 0) ->
+    (forall (n k : nat) (H : 0 < k), k <= n ->
+      P (n - k) k (div (n - k) k H) -> P n k (S (div (n - k) k H))) ->
+        forall (n k : nat) (H : 0 < k), P n k (div n k H).
+Proof.
+  intros. apply divR'_ind; intros.
+    apply H; auto.
+    eapply (divR'_complete _ _ _ H2) in H4. subst. apply H0; assumption.
+    apply divR'_correct with H1. reflexivity.
+Qed.
